
### mono

- `mono` applies a monotonicity rule.
- `mono*` applies monotonicity rules repetitively.
- `mono using x ≤ y` or `mono using [0 ≤ x,0 ≤ y]` creates an assertion for the listed
  propositions. Those help to select the right monotonicity rule.
- `mono left` or `mono right` is useful when proving strict orderings:
   for `x + y < w + z` could be broken down into either
    - left:  `x ≤ w` and `y < z` or
    - right: `x < w` and `y ≤ z`

Here is an example of mono:

```
example (x y z k : ℤ)
  (h : 3 ≤ (4 : ℤ))
  (h' : z ≤ y) :
  (k + 3 + x) - y ≤ (k + 4 + x) - z :=
begin
  mono, -- unfold `(-)`, apply add_le_add
  { -- ⊢ k + 3 + x ≤ k + 4 + x
    mono, -- apply add_le_add, refl
    -- ⊢ k + 3 ≤ k + 4
    mono },
  { -- ⊢ -y ≤ -z
    mono /- apply neg_le_neg -/ }
end
```

More succinctly, we can prove the same goal as:

```
example (x y z k : ℤ)
  (h : 3 ≤ (4 : ℤ))
  (h' : z ≤ y) :
  (k + 3 + x) - y ≤ (k + 4 + x) - z :=
by mono*
```

The same example

### ac_mono

`ac_mono` reduces the `f x ⊑ f y`, for some relation `⊑` and a
monotonic function `f` to `x ≺ y`.

`ac_mono*` unwraps monotonic functions until it can't.

`ac_mono^k`, for some literal number `k` applies monotonicity `k`
times.

`ac_mono h`, with `h` a hypothesis, unwraps monotonic functions and
uses `h` to solve the remaining goal. Can be combined with `*` or `^k`:
`ac_mono* h`

`ac_mono : p` asserts `p` and uses it to discharge the goal result
unwrapping a series of monotonic functions. Can be combined with * or
^k: `ac_mono* : p`

In the case where `f` is an associative or commutative operator,
`ac_mono` will consider any possible permutation of its arguments and
use the one the minimizes the difference between the left-hand side
and the right-hand side.

`ac_mono` can be used as follows:

```
example (x y z k m n : ℕ)
  (h₀ : z ≥ 0)
  (h₁ : x ≤ y) :
  (m + x + n) * z + k ≤ z * (y + n + m) + k :=
begin
  ac_mono,
  -- ⊢ (m + x + n) * z ≤ z * (y + n + m)
  ac_mono,
  -- ⊢ m + x + n ≤ y + n + m
  ac_mono,
end
```

As with `mono*`, `ac_mono*` solves the goal in one go and so does
`ac_mono* h₁`. The latter syntax becomes especially interesting in the
following example:

```
example (x y z k m n : ℕ)
  (h₀ : z ≥ 0)
  (h₁ : m + x + n ≤ y + n + m) :
  (m + x + n) * z + k ≤ z * (y + n + m) + k :=
by ac_mono* h₁.
```

By giving `ac_mono` the assumption `h₁`, we are asking `ac_refl` to
stop earlier than it would normally would.
